proving counter invariants in Epochs.fst

src/tls/Epochs.fst
@@ -88,89 +88,91 @@ let reveal_epochs_inv' (u:unit)
 	     epochs_inv es)
   = ()
 
-let indexable #r #a #p (x:int) (es:MonotoneSeq.i_seq r a p) (h:HH.t) =
-  b2t (x < Seq.length (m_sel h es))
-
-type epoch_ctr_inv (#a:Type0) (#p:(seq a -> Type)) (r:rid) (es:MonotoneSeq.i_seq r a p) =
-  x:int{-1 <= x /\ witnessed (indexable x es)}
+module MS = MonotoneSeq
 
 // Epoch counters i must satisfy -1 <= i < length !es
+type epoch_ctr_inv (#a:Type0) (#p:(seq a -> Type)) (r:rid) (es:MonotoneSeq.i_seq r a p) =
+  x:int{-1 <= x /\ witnessed (MS.int_at_most x es)}
+
 type epoch_ctr (#a:Type0) (#p:(seq a -> Type)) (r:rid) (es:MonotoneSeq.i_seq r a p) = 
   m_rref r (epoch_ctr_inv r es) increases
 
 type epochs (r:rgn) (n:TLSInfo.random) = 
-  | Epochs: es: MonotoneSeq.i_seq r (epoch r n) (fun s -> epochs_inv s) ->
+  | Epochs: es: MonotoneSeq.i_seq r (epoch r n) (epochs_inv #r #n) ->
     	    read: epoch_ctr r es -> 
-	    write: epoch_ctr r es ->
+	    write: epoch_ctr r es -> //NS: probably need some anti-aliasing invariant of these three references
 	    epochs r n  
 
 let containsT (Epochs es r w) (h:HyperHeap.t) =
     MonotoneSeq.i_contains es h 
 
-#set-options "--lax"
+val alloc_log_and_ctrs: #a:Type0 -> #p:(seq a -> Type0) -> r:HH.rid -> 
+  ST (is:MS.i_seq r a p &
+      c1:epoch_ctr r is &
+      c2:epoch_ctr r is)
+     (requires (fun h -> p Seq.createEmpty))
+     (ensures (fun h0 x h1 -> 
+       modifies_one r h0 h1
+       /\ modifies_rref r !{} h0 h1
+       /\ (let (|is, c1, c2|) = x in 
+	  i_contains is h1
+	  /\ m_contains c1 h1
+	  /\ m_contains c2 h1
+	  /\ i_sel h1 is = Seq.createEmpty)))
+let alloc_log_and_ctrs #a #p r = 
+  let init = Seq.createEmpty in 
+  let is = alloc_mref_iseq p r init in 
+  witness is (int_at_most (-1) is); 
+  let c1 : epoch_ctr #a #p r is = m_alloc r (-1) in
+  let c2 : epoch_ctr #a #p r is = m_alloc r (-1) in
+  (| is, c1, c2 |)
 
+val incr_epoch_ctr: #a:Type0 -> #p:(seq a -> Type0) -> #r:HH.rid -> #is:MS.i_seq r a p
+		  -> ctr:epoch_ctr r is
+		  -> ST unit 
+   (requires (fun h -> m_sel h ctr + 1 < Seq.length (i_sel h is)))
+   (ensures (fun h0 _ h1 -> 
+		  modifies_one r h0 h1
+		  /\ modifies_rref r !{as_ref (as_rref ctr)} h0 h1
+		  /\ m_sel h1 ctr = m_sel h0 ctr + 1))
+let incr_epoch_ctr #a #p #r #is ctr = 
+  m_recall ctr;
+  let cur = m_read ctr in 
+  MS.int_at_most_is_stable is (cur + 1);
+  witness is (int_at_most (cur + 1) is);
+  m_write ctr (cur + 1)
+       
 val epochs_init: r:rgn -> n:TLSInfo.random -> ST (epochs r n)
        (requires (fun h -> True))
-       (ensures (fun h0 x h1 -> True))
-let epochs_init (r:rgn) (n:TLSInfo.random) = 
-    let esref = MonotoneSeq.alloc_mref_seq r Seq.createEmpty in
-    m_recall esref;
-    witness esref (fun h -> -1 < Seq.length (m_sel h esref));
-    let x : epoch_ctr_inv #_ #(fun s -> epochs_inv s) r esref = -1 in
-    let mr = m_alloc r x in
-    let mw = m_alloc r x in
-    Epochs esref mr mw
+       (ensures (fun h0 x h1 -> modifies_one r h0 h1 /\ modifies_rref r !{} h0 h1))
+let epochs_init (r:rgn) (n:TLSInfo.random) =
+  let (| esref, c1, c2 |) = alloc_log_and_ctrs #(epoch r n) #(epochs_inv #r #n) r in
+  Epochs esref c1 c2
 
-val add_epoch: #r:rgn -> #n:TLSInfo.random -> 
-    	       es:epochs r n -> e: epoch r n -> ST unit
-       (requires (fun h -> True))
-       (ensures (fun h0 x h1 -> True))
-let add_epoch #rg #n (Epochs es r w) e = 
-    MonotoneSeq.i_write_at_end #rg es e
+inline let incr_pre #r #n (es:epochs r n) (proj:(es:epochs r n -> Tot (epoch_ctr r (Epochs.es es)))) h : GTot Type0 = 
+  let ctr = proj es in 
+  let cur = m_sel h ctr in
+  cur + 1 < Seq.length (i_sel h (Epochs.es es))
 
-val incr_reader: #r:rgn -> #n:TLSInfo.random ->
-               es:epochs r n -> ST unit
-       (requires (fun h ->
-         let Epochs mes mr _ = es in
-         let cur = m_sel h mr in
-         cur + 1 < Seq.length (m_sel h mes)))
-       (ensures (fun h0 () h1 ->
-         let Epochs mes mr _ = es in
-         let oldr = m_sel h0 mr in
-         let newr = m_sel h1 mr in
-         modifies (Set.singleton r) h0 h1
-         /\ HH.modifies_rref r !{HH.as_ref (as_rref mr)} h0 h1
-         /\ newr = oldr + 1
-         /\ witnessed (fun h -> -1 <= newr /\ newr < Seq.length (m_sel h mes))))
-let incr_reader #r #n (Epochs es mr _) =
-  m_recall mr; m_recall es;
-  let cur = m_read mr in
-  witness es (indexable (cur+1) es);
-  m_write mr (cur + 1)
+inline let incr_post #r #n (es:epochs r n) (proj:(es:epochs r n -> Tot (epoch_ctr r (Epochs.es es)))) h0 (_:unit) h1 : GTot Type0 = 
+  let ctr = proj es in 
+  let oldr = m_sel h0 ctr in
+  let newr = m_sel h1 ctr in
+  modifies_one r h0 h1
+  /\ HH.modifies_rref r !{HH.as_ref (as_rref ctr)} h0 h1
+  /\ newr = oldr + 1
 
-val incr_writer: #r:rgn -> #n:TLSInfo.random ->
-               es:epochs r n -> ST unit
-       (requires (fun h ->
-         let Epochs mes _ mw = es in
-         let cur = m_sel h mw in
-         cur + 1 < Seq.length (m_sel h mes)))
-       (ensures (fun h0 () h1 ->
-         let Epochs mes _ mw= es in
-         let oldw = m_sel h0 mw in
-         let neww = m_sel h1 mw in
-         modifies (Set.singleton r) h0 h1
-         /\ HH.modifies_rref r !{HH.as_ref (as_rref mw)} h0 h1
-         /\ neww = oldw + 1
-         /\ witnessed (fun h -> -1 <= neww /\ neww < Seq.length (m_sel h mes))))
-let incr_writer #r #n (Epochs es _ mw) =
-  m_recall mw; m_recall es;
-  let cur = m_read mw in
-  witness es (indexable (cur+1) es);
-  m_write mw (cur + 1)
+let incr_reader #r #n (es:epochs r n) : ST unit
+    (requires (incr_pre es Epochs.read))
+    (ensures (incr_post es Epochs.read))
+    = incr_epoch_ctr (Epochs.read es)
 
-#reset-options
+let incr_writer #r #n (es:epochs r n) : ST unit
+    (requires (incr_pre es Epochs.write))
+    (ensures (incr_post es Epochs.write))
+    = incr_epoch_ctr (Epochs.write es)
 
-let get_epochs (Epochs es r w) = es 
+let get_epochs (Epochs es r w) = es
 
 let epochsT (Epochs es r w) (h:HyperHeap.t) = MonotoneSeq.i_sel h es
 
